By default, avoid guard-holders removal inside hide.  Add comment to HIDE terms saying which constrained function is to blame for failed evaluation.
Quoting :doc note-8-3:

  The algorithm for removing [guard-holders] has been modified to avoid
  diving into calls of [hide].  However, it is possible to obtain the
  former behavior; see [guard-holders].

  Since its earliest years, ACL2 uses evaluation to simplify ground
  terms (terms with no free variables).  ACL2 would sometimes
  generate a call of [hide] around a term that fails to evaluate
  because of an attempt to call a constrained function.  Now, that
  call incorporates a comment saying which constrained function is
  responsible for the failure.  See [comment].

In addition to completion of the usual "everything" regression
successfully, the "devel-check" process completed successfully.

doc.lisp
@@ -3079,6 +3079,9 @@ Subtopics
   [Coerce]
       Coerce a character list to a string and a string to a list
 
+  [Comment]
+      Variant of [prog2$] to help debug evaluation failures during proofs
+
   [Comp]
       Compile some ACL2 functions
 
@@ -17513,6 +17516,75 @@ Subtopics
 
   [Save-exec]
       Save an executable image and a wrapper script")
+ (COMMENT
+  (HIDE ACL2-BUILT-INS)
+  "Variant of [prog2$] to help debug evaluation failures during proofs
+
+  Semantically, (comment x y) equals y; the value of x is ignored.
+  Thus comment is much like [prog2$].  However, when you see a call
+  of comment in ACL2 proof output, it will likely be under a call of
+  [hide], with information that may be helpful in understanding why
+  the call of hide was inserted.  Consider the following example.
+
+    (defstub f (x) t)
+    (defun g (x) (cons (f x) x))
+    (defun h (x) (cons x (cdr (g x))))
+    (thm (equal (h 3) '(3 . 3)))
+
+  The proof attempt fails for the [thm] call, indicating the checkpoint
+  shown below.
+
+    *** Key checkpoint at the top level: ***
+
+    Goal'
+    (EQUAL (HIDE (COMMENT \"Called constrained function F\" (H 3)))
+           '(3 . 3))
+
+  The first argument of equal is logically just (h 3).  But the comment
+  and hide wrappers are telling us that evaluation of (h 3) failed
+  because it led to a call of the constrained function f.  It is easy
+  to see why in this case, by looking at the definitions, where h
+  calls g, which calls f.  But more complicated such failures may be
+  difficult to understand without such information.  In very
+  complicated cases, one might even want to use the Lisp debugger
+  after designating a [break$] call using [trace$], like this (here,
+  shown using host Lisp CCL).
+
+    ACL2 !>(trace$ (f :entry (break$)))
+     ((F :ENTRY (BREAK$)))
+    ACL2 !>(thm (equal (h 3) '(3 . 3)))
+
+    > Break: Break
+    > While executing: BREAK$, in process listener(1).
+    > Type :GO to continue, :POP to abort, :R for a list of available restarts.
+    > If continued: Return from BREAK.
+    > Type :? for other options.
+    1 > :b ; user input to get backtrace
+     (262932A0) : 0 (BREAK$) 157
+     (262932F0) : 1 (F 3) 141
+     (26293338) : 2 (FUNCALL #'#<(:INTERNAL ACL2_*1*_ACL2::G ACL2_*1*_ACL2::G)> 3) 37
+     (26293350) : 3 (FUNCALL #'#<(:INTERNAL ACL2_*1*_ACL2::H ACL2_*1*_ACL2::H)> 3) 37
+     (26293368) : 4 (RAW-EV-FNCALL H (3) NIL NIL [[.. output elided ..]]
+
+  This output from Lisp is quite low-level, but reading from the bottom
+  up provides the following sequence of events.
+
+    * 4. Call h with argument list (3).
+    * 3. Call the [executable-counterpart] of h.
+    * 2. Call the [executable-counterpart] of g.
+    * 1. Attempt to call the constrained function, f.
+
+  An easy way to avoid this proof failure is to avoid execution of
+  calls of h and g, as follows.
+
+    (thm (equal (h 3) '(3 . 3))
+         :hints ((\"Goal\" :in-theory (disable (:e g) (:e h)))))
+
+  (It actually suffices to disable only (:e h), but the workings of the
+  ACL2 rewriter are out of scope here.)
+
+  Also see [hide] for further discussion of how to avoid such proof
+  failures.")
  (COMMON-LISP
   (ABOUT-ACL2)
   "Relation to Common Lisp, including deviations from the spec
@@ -32249,11 +32321,13 @@ Subtopics
   the executable-counterpart of a function.  For discussion of
   executable-counterparts of functions, see [evaluation].
 
-    Examples:
+    Example:
     (:executable-counterpart length)
 
-  which may be abbreviated in [theories] as
+  which may be abbreviated in [theory] expressions in either of the
+  following two ways (see [rune]).
 
+    (:e length)
     (length)
 
   Every [defun] introduces at least two rules used by the theorem
@@ -41196,7 +41270,15 @@ Subtopics
   Because of how [mbe] and [ec-call] are defined in terms of
   [return-last], the expressions (mbe :logic l :exec e) and (ec-call
   (f t1 ... tk)) are effectively transformed by removing guard
-  holders into l and (f t1 ... tk), respectively.")
+  holders into l and (f t1 ... tk), respectively.
+
+  Note that by default, guard-holders are not removed inside calls of
+  [hide].  You can however cause them to be removed inside such calls
+  after all, as was the case through Version 8.2, as follows.
+
+    (defattach-system ; generates (local (defattach ...))
+      remove-guard-holders-blocked-by-hide-p
+      constant-nil-function-arity-0)")
  (GUARD-INTRODUCTION
   (GUARD)
   "Introduction to [guard]s in ACL2
@@ -42247,7 +42329,9 @@ Subtopics
   rest of the goal, if that goal (or a subgoal of it) fails to be
   proved.
 
-  Hide terms are also ignored by the induction heuristics.
+  Hide terms are generally ignored not only by the rewriter but by
+  other ACL2 procedures, including the induction heuristics and (by
+  default) removal of [guard-holders].
 
   Sometimes the ACL2 simplifier inserts hide terms into a proof attempt
   out of the blue, as it were.  Why and what can you do about it?
@@ -42259,28 +42343,35 @@ Subtopics
           (constrained-fn x y z)
           t))
 
-  Suppose the term (another-fn 'a 'b 'c) arises in a proof.  Since the
-  arguments are all constants, ACL2 will try to reduce such a term to
+  Suppose the term (another-fn 1 2 3) arises in a proof.  Since the
+  arguments are all constants, ACL2 may try to reduce such a term to
   a constant by executing the definition of another-fn.  However,
   after a possibly extensive computation (because of big-hairy-test)
   the execution fails because of the unevaluable call of
   constrained-fn.  To avoid subsequent attempts to evaluate the term,
-  ACL2 embeds it in a hide expression, i.e., rewrites it to (hide
-  (another-fn 'a 'b 'c)).
+  ACL2 embeds it in a hide expression.  Typically that expression
+  will use a call of [comment], where (comment x y) is logically just
+  y, to tell you the problematic constrained function, in this case
+  by rewriting the original expression to:
+
+    (hide (comment \"Called constrained function CONSTRAINED-FN\"
+                   (another-fn 1 2 3))).
 
   You might think this rarely occurs since all the arguments of
   another-fn must be constants.  You would be right except for one
   special case: if another-fn takes no arguments, i.e., is a constant
   function, then every call of it fits this case.  Thus, if you
-  define a function of no arguments in terms of a constrained
-  function, you will often see (another-fn) rewrite to (hide
-  (another-fn)).
+  define a function f of no arguments in terms of a constrained
+  function g, you may often see (f) rewrite to:
 
-  We do not hide the term if the executable-counterpart of the function
-  is disabled --- because we do not try to evaluate it in the first
-  place.  Thus, to prevent the insertion of a hide term into the
-  proof attempt, you can globally disable the executable-counterpart
-  of the offending defined function, e.g.,
+    (hide (comment \"Called constrained function G\"
+                   (f))).
+
+  We do not hide the term if the [executable-counterpart] of the
+  function is [disable]d --- because we do not try to evaluate it in
+  the first place.  Thus, to prevent the insertion of a hide term
+  into the proof attempt, you can globally disable the
+  executable-counterpart of the offending defined function, e.g.,
 
     (in-theory (disable (:executable-counterpart another-fn))).
 
@@ -42293,10 +42384,11 @@ Subtopics
   the proof of some theorem, thm, it is necessary to leave the
   executable-counterpart of another-fn enabled but that the call
   (another-fn 1 2 3) arises in the proof and cannot be computed.
-  Thus the proof attempt will introduce the term (hide (another-fn 1
-  2 3)).  Suppose that you can show that (another-fn 1 2 3) is
-  (constrained-fn 1 2 3) and that such a step is necessary to the
-  proof.  Unfortunately, proving the rewrite rule
+  Thus the proof attempt will introduce the term (hide (comment \"..\"
+  (another-fn 1 2 3))) mentioned above.  Suppose that you can show
+  that (another-fn 1 2 3) is (constrained-fn 1 2 3) and that such a
+  step is necessary to the proof.  Unfortunately, proving the rewrite
+  rule
 
     (defthm thm-helper
       (equal (another-fn 1 2 3) (constrained-fn 1 2 3)))
@@ -42305,22 +42397,25 @@ Subtopics
   inside the hide.  However,
 
     (defthm thm-helper
-      (equal (hide (another-fn 1 2 3)) (constrained-fn 1 2 3)))
+      (equal (hide (comment \"Called constrained function CONSTRAINED-FN\"
+                            (another-fn 1 2 3)))
+             (constrained-fn 1 2 3)))
 
   would be applied in the proof of thm and is the rule you should
   prove.
 
   Now to prove thm-helper you need to use the two ``tricks'' which have
   already been discussed.  First, to eliminate the hide term in the
-  proof of thm-helper you should include the hint :expand (hide
-  (another-fn 1 2 3)).  Second, to prevent the hide term from being
-  reintroduced when the system tries and fails to evaluate
-  (another-fn 1 2 3) you should include the hint :in-theory (disable
-  (:executable-counterpart another-fn)).  Thus, thm-helper will
-  actually be:
+  proof of thm-helper you should include a hint to :expand that term.
+  Second, to prevent the hide term from being reintroduced when the
+  system tries and fails to evaluate (another-fn 1 2 3) you should
+  include the hint :in-theory (disable (:executable-counterpart
+  another-fn)).  Thus, thm-helper will actually be:
 
     (defthm thm-helper
-      (equal (hide (another-fn 1 2 3)) (constrained-fn 1 2 3))
+      (equal (hide (comment \"Called constrained function CONSTRAINED-FN\"
+                            (another-fn 1 2 3)))
+             (constrained-fn 1 2 3))
       :hints
       ((\"Goal\" :expand (hide (another-fn 1 2 3))
                :in-theory (disable (:executable-counterpart another-fn)))))
@@ -42332,7 +42427,13 @@ Subtopics
 
     (defun hide (x)
            (declare (xargs :guard t))
-           x)")
+           x)
+
+
+Subtopics
+
+  [Comment]
+      Variant of [prog2$] to help debug evaluation failures during proofs")
  (HINTS
   (MISCELLANEOUS)
   "Advice to the theorem proving process
@@ -83409,6 +83510,17 @@ Changes to Existing Features
   An undocumented kind of [fake-rune] is no longer reported by
   [show-accumulated-persistence].  Thanks to Eric Smith for bringing
   this issue to our attention.
+
+  The algorithm for removing [guard-holders] has been modified to avoid
+  diving into calls of [hide].  However, it is possible to obtain the
+  former behavior; see [guard-holders].
+
+  Since its earliest years, ACL2 uses evaluation to simplify ground
+  terms (terms with no free variables).  ACL2 would sometimes
+  generate a call of [hide] around a term that fails to evaluate
+  because of an attempt to call a constrained function.  Now, that
+  call incorporates a comment saying which constrained function is
+  responsible for the failure.  See [comment].
 
 
 New Features
